dist/SizeClassSelection.h
@@ -12,6 +12,8 @@ uint32_t SizeClassSelection_log2u64(uint64_t x);
 
 krml_checked_int_t SizeClassSelection_sort(krml_checked_int_t x);
 
+uint32_t SizeClassSelection_log2u64_ceil(uint64_t x);
+
 uint32_t SizeClassSelection_inv_impl(uint32_t bound_input, uint32_t bound_len, uint32_t x);
 
 
